make cbor_match_serialized_payload_* consistent

src/cbor/raw/pulse/everparse/CBOR.Pulse.Raw.Match.Serialized.fst
@@ -7,16 +7,16 @@ module U64 = FStar.UInt64
 
 let cbor_match_serialized_payload_array
   c p r
-= exists* r' .
-    pts_to_serialized (tot_serialize_nlist (U64.v c.cbor_serialized_header.value)  serialize_raw_data_item) c.cbor_serialized_payload #(p `perm_mul` c.cbor_serialized_perm) r' **
+= exists* n (r': nlist n raw_data_item) .
+    pts_to_serialized (tot_serialize_nlist n serialize_raw_data_item) c #p r' **
     pure (r == r')
 
 let cbor_match_serialized_payload_map
   c p r
-= exists* r' .
-    pts_to_serialized (tot_serialize_nlist (U64.v c.cbor_serialized_header.value)  (serialize_raw_data_item `tot_serialize_nondep_then` serialize_raw_data_item)) c.cbor_serialized_payload #(p `perm_mul` c.cbor_serialized_perm) r' **
+= exists* n (r' : nlist n (raw_data_item & raw_data_item)) .
+    pts_to_serialized (tot_serialize_nlist n (serialize_raw_data_item `tot_serialize_nondep_then` serialize_raw_data_item)) c #p r' **
     pure (r == r')
 
 let cbor_match_serialized_payload_tagged
   c p r
-= pts_to_serialized serialize_raw_data_item c.cbor_serialized_payload #(p `perm_mul` c.cbor_serialized_perm) r
+= pts_to_serialized serialize_raw_data_item c #p r
