src/cbor/raw/pulse/CBOR.Pulse.Raw.Match.Serialized.fsti
@@ -8,19 +8,19 @@ module U8 = FStar.UInt8
 module SZ = FStar.SizeT
 
 val cbor_match_serialized_payload_array
-  (c: cbor_serialized)
+  (c: slice U8.t)
   (p: perm)
   (r: list raw_data_item)
 : Tot slprop
 
 val cbor_match_serialized_payload_map
-  (c: cbor_serialized)
+  (c: slice U8.t)
   (p: perm)
   (r: list (raw_data_item & raw_data_item))
 : Tot slprop
 
 val cbor_match_serialized_payload_tagged
-  (c: cbor_serialized)
+  (c: slice U8.t)
   (p: perm)
   (r: raw_data_item)
 : Tot slprop
